<section xml:id="section-chain-rule">
  <title>The Chain Rule</title>
  <subsection xml:id="subsection-derivatives-composition">
    <title>Derivatives of Compositions</title>
    <p>
      The rules we have so far give us the tools to calculate many
      derivatives. However, they don't address composition. How do
      we differentiate <m>\sin x^2</m>?  The rule that addresses
      derivatives of composed functions is called the chain rule. The
      chain rule has two notations. Let <m>f</m> and <m>g</m> be
      differentiable functions and consider the composition
      <m>f(g(x))</m>. It is often useful to label <m>g(x)</m> by a
      new, temporary variable <m>u = g(x)</m>. The vertical line mean
      evaluate by replaing <m>u</m> with <m>g(x)</m>. 
      <me>
        \frac{d}{dx} f(g(x)) = f^\prime(g(x)) g^\prime(x) = \left.
        \frac{df(u)}{du} \right|_{u=g(x)} \frac{dg}{dx} 
      </me>
    </p>
    <p>
      The variety of notations is somewhat due to the difficult nature
      of the rule<mdash />it's hard to clearly describe. The key idea
      is to think of composition in terms of inside and outside
      functions. The derivative of the composition is the derivative
      of the outside (<m>f^\prime</m>) evaluted at the inside
      (<m>f^\prime(g(x))</m>), then multiplied by the derivative of
      the inside (<m>g^\prime</m>). There is one other way of
      expressing the chain rule.
      <me>
        \frac{df}{dx} = \frac{df}{dg} \frac{dg}{dx}
      </me>
    </p>
    <p>
      In this last version of the chain rule, we can think of the
      infinitesimals <m>df</m>, <m>dg</m> and <m>dx</m> as something
      like fractions in Leibniz notation (<m>\frac{df}{dx}</m>).
      These terms are not fractions, but they act a bit like fractions.
    </p>
    <p>
      The proof of the chain rule is tricky, but the following
      argument gives the idea. The argument is a little imprecise in
      the fourth step, where we replace <m>g(x)</m> with the temporary
      variable <m>u</m>, since we haven't established that such an
      operation is valid. In the proof, let <m>F = f \circ g</m>.
      <md>
        <mrow>
          \frac{dF}{dx}(a) \amp = \lim_{x \rightarrow a} \frac{f
          \circ g (x) - f \circ g(a)}{x-a} = \lim_{x \rightarrow a}
          \frac{f(g(x)) - f(g(a))}{x-a}
        </mrow>
        <mrow>
          \amp = \lim_{x \rightarrow a} \frac{f(g(x)) - f(g(a))}{g(x)
          - g(a)} \frac{g(x) - g(a)}{x-a}
        </mrow>
        <mrow>
          \amp = \lim_{x \rightarrow a} \frac{f(g(x)) - f(g(a))}{g(x)
          - g(a)} \lim_{x \rightarrow a} \frac{g(x) - g(a)}{x-a}
        </mrow>
        <mrow>
          \amp = \lim_{u \rightarrow g(a)} \frac{f(u) - f(g(a))}{u -
          g(a)} \lim_{x \rightarrow a} \frac{g(x) - g(a)}{x-a}
        </mrow>
        <mrow>
          \amp = \left. \frac{df}{du} \right|_{u=g(a)} \left.
          \frac{dg}{dx} \right|_{x=a} = f^\prime(g(a)) g^\prime(a)
        </mrow>
      </md>
    </p>
    <example>
      <statement>
        <md>
          <mrow>
            \frac{d}{dx} e^{ax} \amp = ae^{ax}
          </mrow>
          <mrow>
            \frac{d}{dx} \sin 3x \amp = 3 \cos 3x
          </mrow>
          <mrow>
            \frac{d}{dx} e^{x^2+2} \amp = (2x) e^{x^2+2}
          </mrow>
          <mrow>
            \frac{d}{dx} e^{e^x} \amp = e^x e^{e^x}
          </mrow>
          <mrow>
            \frac{d}{dx} \sin \left( \frac{x^2+1}{x^2-1} \right) \amp
            = \cos \left( \frac{x^2+1}{x^2-1} \right) \frac{d}{dx}
            \frac{x^2+1}{x^2-1}
          </mrow>
          <mrow>
            \amp = \cos \left( \frac{x^2+1}{x^2-1} \right)
            \frac{(x^2-1) \frac{d}{dx} (x^2+1) - (x^2+1) \frac{d}{dx}
            (x^2-1)}{(x^2-1)^2}
          </mrow>
          <mrow>
            \amp = \cos \left( \frac{x^2+1}{x^2-1} \right)
            \frac{(x^2-1) (2x) - (x^2+1) (2x)}{(x^2-1)^2}
          </mrow>
          <mrow>
            \amp = \cos \left( \frac{x^2+1}{x^2-1} \right)
            \frac{2x(x^2-1 - x^2 -1)}{(x^2-1)^2} 
          </mrow>
          <mrow>
            \amp = - \cos \left(
            \frac{x^2+1}{x^2-1} \right) \frac{4x}{(x^2-1)^2}
          </mrow>
          <mrow>
            \frac{d}{dx} \cos ( e^{\sin x}) \amp = -\sin (e^{\sin x})
            \frac{d}{dx} e^{\sin x} = -\sin (e^{\sin x}) e^{\sin x}
            \frac{d}{dx} \sin x 
          </mrow>
          <mrow>
            \amp = -\sin (e^{\sin x}) e^{\sin x} \cos
          </mrow>
        </md>
      </statement>
    </example>
    <example>
      <statement>
        <p>
          We can use the chain rule to differentiate arbitrary
          exponential functions in more detail than before:
          <md>
            <mrow>
              \frac{d}{dx} a^x\amp = \frac{d}{dx} e^{x\ln a} = e^{x
              \ln a} \ln a = a^x \ln a
            </mrow>
          </md>
        </p>
      </statement>
    </example>
    <example>
      <statement>
        <p>
          We can also use the chain rule with a neat little
          exponential trick to differentiate <m>f(x) = x^x</m>. (In
          this calculation, we use <m>\frac{d}{dx} \ln x =
          \frac{1}{x}</m>, which we will prove in the next section.)
          <md>
            <mrow>
              \frac{d}{dx} x^x \amp = \frac{d}{dx} e^{x\ln x} =
              e^{x\ln x} \frac{d}{dx} x\ln x = x^x (\ln x \frac{d}{dx}
              x + x \frac{d}{dx} \ln x) = x^x(\ln x + 1)
            </mrow>
          </md>
        </p>
      </statement>
    </example>
    <example>
      <statement>
        <p>
          We can use the chain rule to prove the quotient rule.
          <md>
            <mrow>
              \frac{d}{dx} \frac{f}{g} \amp = \frac{d}{dx} f g^{-1} =
              f \frac{d}{dx} g^{-1} + g^{-1} \frac{d}{dx} = -f g^{-2}
              \frac{dg}{dx} + g^{-1} \frac{df}{dx} = \frac{gf^\prime -
              fg^\prime}{g^2}
            </mrow>
          </md>
        </p>
      </statement>
    </example>
  </subsection>
  <subsection xml:id="subsection-derivatives-inverse-functions">
    <title>Derivatives of Inverse Functions</title>
    <p>
      We just used the rule <m>\frac{d}{dx} \ln x = \frac{1}{x}</m>
      without justification. What is this justification?  The
      logarithm is the inverse of the exponential, which leads us to
      thinking about the derivatives of inverse functions. There is a
      rule for such derivatives. Let's write <m>x = f \circ
      f^{-1}(x)</m>, differentiate both sides using the chain rule,
      and rearrange to get an expression for <m>\frac{d}{dx}
      f^{-1}(x)</m>.
      <md>
        <mrow>
          1 \amp = \frac{d}{dx} x = \frac{d}{dx} f \circ f^{-1} =
          f^\prime ( f^{-1}(x)) \frac{d}{dx} f^{-1}(x)
        </mrow>
        <mrow>
          \frac{d}{dx} f^{-1}(x) \amp =
          \frac{1}{f^\prime(f^{-1}(x))}
        </mrow>
      </md>
    </p>
    <p>
      Then we can prove the derivative formula we just used for <m>\ln
      x</m>.
      <me>
        \frac{d}{dx} \ln x = \frac{1}{e^{\ln x}} = \frac{1}{x}
      </me>
    </p>
    <p>
      We can also prove derivative rules for the inverse trig
      functions.
      <md>
        <mrow>
          \frac{d}{dx} \arccos x \amp = \frac{1}{-\sin(\arccos x)} =
          \frac{-1}{\sqrt{1-\cos^2(\arccos x)}} =
          \frac{-1}{\sqrt{1-x^2}}
        </mrow>
        <mrow>
          \frac{d}{dx} \arcsin x \amp = \frac{1}{\cos(\arcsin x)} =
          \frac{1}{\sqrt{1-\sin^2(\arcsin x)}} =
          \frac{1}{\sqrt{1-x^2}}
        </mrow>
        <mrow>
          \frac{d}{dx} \arctan x \amp = \frac{1}{\sec^2(\arctan x)} =
          \frac{1}{1+\tan^2(\arctan x)} = \frac{1}{1+x^2}
        </mrow>
      </md>
    </p>
    <example>
      <statement>
        <md>
          <mrow>
            \frac{d}{dx} \ln(x^2+1) \amp = \frac{1}{x^2+1}
            \frac{d}{dx} x^2+1 = \frac{2x}{x^2+1}
          </mrow>
          <mrow>
            \frac{d}{dx} \ln (x + 3x \arcsin x) \amp =
            \frac{1}{x+3\arcsin x} \left( 1 + 3\arcsin x +
            \frac{3x}{\sqrt{1-x^2}} \right)
         </mrow>
        </md>
      </statement>
    </example>
    <example>
      <statement>
        <p>
          Usually, when we differentiate, we get complicated
          expressions which we can't simplify into nice forms. Every
          now and then, we have an example that allows a very nice
          simplifcation.
          <md>
            <mrow>
              \amp \frac{d}{dx} \left( \frac{x}{2} \sqrt{x^2-9} -
              \frac{9}{2} \ln( x + \sqrt{x^2-9} ) \right) 
            </mrow>
            <mrow>
              \amp = \frac{\sqrt{x^2-9}}{2} + \frac{x
              2x}{4\sqrt{x^2-9}} - \frac{9}{2} \frac{1}{x+
              \sqrt{x^2-9}} \left( 1 + \frac{2x}{2\sqrt{x^2-9}}
              \right)
            </mrow>
            <mrow>
              \amp = \frac{\sqrt{x^2-9}}{2} +
              \frac{x^2}{2\sqrt{x^2-9}} - \frac{9}{2} \frac{2
              \sqrt{x^2-9} + 2x}{2\sqrt{x^2-9}(x+ \sqrt{x^2-9})}
            </mrow>
            <mrow>
              \amp = \frac{\sqrt{x^2-9}}{2} +
              \frac{x^2}{2\sqrt{x^2-9}} - \frac{9}{2}
              \frac{\sqrt{x^2-9} + x}{\sqrt{x^2-9}(x+ \sqrt{x^2-9})}
            </mrow>
            <mrow>
              \amp = \frac{\sqrt{x^2-9}}{2} +
              \frac{x^2-9}{2\sqrt{x^2-9}}
            </mrow>
            <mrow>
              \amp = \frac{\sqrt{x^2-9}}{2} +
              \frac{\sqrt{x^2-9}}{2} = \sqrt{x^2-9}
            </mrow>
          </md>
        </p>
      </statement>
    </example>
  </subsection>
</section>
