<section xml:id="section-des">
  <title>Solving Differential Equations</title>
  <subsection xml:id="subsection-direct-integration">
    <title>Solving By Direct Integration</title>
    <p>
      Early in the course, we talked about differential equations in
      order to understand derivatives as rates of changes. We looked
      at autonomous differential equations, particularly for
      populations models, and we used the qualitative technique of
      phase-line analysis to understand them.
    </p>
    <p>
      Now that we can calculate derivatives and integrals in some
      detail, we can return to differential equations. With these
      techniques, we'll actually try to solve the DEs, instead of
      using a qualitative approach. In the easiest case, the right
      side of a DE only involves the independant variable.
      <me>
        \frac{df}{dx} = g(x)
      </me>
    </p>
    <p>
      Since only the independant variable <m>x</m> appears on the
      right side, we can simply integrate both sides in <m>x</m>.
      <me>
        \int \frac{df}{dx} dx = \int g(x) dx
      </me>
    </p>
    <p>
      On the left, the integral of the derivative is the original
      funciton <m>f</m>.
      <me>
        f(x) = \int g(x) dx
      </me>
    </p>
  </subsection>
  <subsection xml:id="subsection-ivps">
    <title>Initial Value Problems</title>
    <p>
      When we integrate to solve a DE, we will get a constant of
      integration. In order to determine that constant, we are often
      given an initial condition, such as <m>f(0) = 0</m>.
      Differential equations problems with initial conditions are
      often called <em>initial value problems</em> (IVPs).
    </p>
    <example>
      <statement>
        <md>
          <mrow>
            \frac{df}{dx} \amp = x^3 \amp \amp   f(0) = 7
          </mrow>
          <mrow>
            \int \frac{df}{dx} dx \amp = \int x^3 dx \amp \amp 
          </mrow>
          <mrow>
            f \amp = \frac{x^4}{4} + c \amp \amp 
          </mrow>
          <mrow>
            7 \amp = \frac{0^4}{4} + c \implies c = 7 \amp \amp 
          </mrow>
          <mrow>
            f(x) \amp = \frac{x^4}{4} + 7 \amp \amp 
          </mrow>
        </md>
      </statement>
    </example>
    <example>
      <statement>
        <md>
          <mrow>
            \frac{df}{dt} \amp = 6 \sin 3t \amp \amp f \left(
            \frac{\pi}{6} \right) = 6
          </mrow>
          <mrow>
            \int \frac{df}{dt} dt \amp = \int 6 \sin 3t dt \amp \amp 
          </mrow>
          <mrow>
            f(x) \amp = \int 6 \sin 3t dt = -2\cos 3t + c \amp \amp 
          </mrow>
          <mrow>
            6 \amp = -2\cos \frac{\pi}{2} + c = 0 + c \implies c=6
            \amp \amp 
          </mrow>
          <mrow>
            f(x) \amp = -2 \cos 3t + 6 \amp \amp
          </mrow>
        </md>
      </statement>
    </example>
    <example>
      <statement>
        <md>
          <mrow>
            \frac{df}{dx} \amp = \frac{1}{x^2+1} \amp \amp f(1) = \pi
          </mrow>
          <mrow>
            \int \frac{df}{dx} dx \amp = \int \frac{1}{x^2+1} dx \amp
            \amp 
          </mrow>
          <mrow>
            f \amp = \int \frac{1}{x^2+1} dx = \arctan x + c \amp \amp 
          </mrow>
          <mrow>
            \pi \amp = \arctan(1) + c = \frac{\pi}{4} + c \implies c
            = \frac{3\pi}{4} \amp \amp 
          </mrow>
          <mrow>
            f(x) \amp = \arctan x + \frac{3\pi}{4} \amp \amp
          </mrow>
        </md>
      </statement>
    </example>
  </subsection>
  <subsection xml:id="subsection-seperable">
    <title>Seperable Differential Equations</title>
    <p>
      Solving DEs is a very difficult task in general; the previous
      examples were all artificially simple. For this course, we're
      going to restrict to a specific type of DE called a seperable
      equation. Let <m>f(x)</m> and <m>g(y)</m> be continuous
      functions in <m>x</m> and <m>y</m>, respectively. Seperable
      differential equations are DEs where the dependent and
      independent variable can be seperated.
      <me>
        \frac{dy}{dx} = f(x) g(y)
      </me>
    </p>
    <p>
      In particular, this includes the autonomous equations we
      previously studied; if we set <m>f=1</m> then we get an
      autonomous equation.
    </p>
    <p>
      To solve these equations, take <m>g(y)</m> to the left side of
      the equation and then integrate in <m>x</m>. 
      <md>
        <mrow>
          \frac{1}{g(y)} \frac{dy}{dx} \amp = f(x)
        </mrow>
        <mrow>
          \int \frac{1}{g(y)} \frac{dy}{dx} dx \amp = f(x) dx
        </mrow>
      </md>
    </p>
    <p>
      With a substitution <m>y = y(x)</m> (so that <m>dy =
      \frac{dy}{dx} dx</m>), we can change the left side
      of the integral into an integral in <m>y</m>. (This looks
      strange, but it's really decided to treat <m>y</m> as a
      variable, instead of as a function <m>y(x)</m>). 
      <me>
        \int \frac{1}{g(y)} dy = \int f(x) dx + c 
      </me>
    </p>
    <p>
      We have now seperated the problem into two integrals, hence
      calling these seperable equation. Now we try to integrate both
      sides. After the integration is complete, we try to solve for
      <m>y</m> as a function of <m>x</m>. If we can, that function is
      the solution. Often we can't, and we leave the result as an
      implicit expression in <m>x</m> and <m>y</m>. We do need a
      constant of integration (which I wrote as <m>c</m>, but it is
      sufficient to include it on just one side of the equation. 
    </p>
    <example>
      <statement>
        <md>
          <mrow>
            \frac{dy}{dx} \amp = \frac{\sin x}{y} \amp \amp y(0) = 1
          </mrow>
          <mrow>
            \int y dy \amp = \int \sin x dx \amp \amp 
          </mrow>
          <mrow>
            \frac{y^2}{2} \amp = - \cos x + c \amp \amp 
          </mrow>
          <mrow>
            \frac{1^2}{2} \amp = - \cos 0 + c \implies c =
            \frac{3}{2} \amp \amp 
          </mrow>
          <mrow>
            \frac{y^2}{2} \amp = - \cos x + \frac{3}{2} \amp \amp 
          </mrow>
          <mrow>
            y \amp = \pm \sqrt{ 2 \left( \frac{3}{2} - \cos x \right)}
            = \pm \sqrt{3 - 2 \cos x} 
          </mrow>
        </md>
      </statement>
    </example>
    <example>
      <statement>
        <md>
          <mrow>
            \frac{dy}{dx} \amp = \frac{-x}{y} \amp \amp y(4) = 3 
          </mrow>
          <mrow>
            \int y dy \amp = - \int x dx \amp \amp 
          </mrow>
          <mrow>
            \frac{y^2}{2} \amp = \frac{-x^2}{2} + c \amp \amp 
          </mrow>
          <mrow>
            y^2 + x^2 \amp = c \amp \amp 
          </mrow>
          <mrow>
            4^2 + 3^2 \amp = c \implies c = 25 \amp \amp 
          </mrow>
          <mrow>
            y^2 + x^2 \amp = 25 \amp \amp 
          </mrow>
          <mrow>
            y \amp = \pm \sqrt{25 - x^2} 
          </mrow>
        </md>
      </statement>
    </example>
    <example>
      <statement>
        <md>
          <mrow>
            \frac{dy}{dx} \amp = y^2 + 1 \amp \amp y(0) = 0 
          </mrow>
          <mrow>
            \int \frac{1}{y^2+1} dy \amp = \int 1 dx \amp \amp 
          </mrow>
          <mrow>
            \arctan y \amp = x + c \amp \amp
          </mrow>
          <mrow>
            y \amp = \tan (x + c) \amp \amp 
          </mrow>
          <mrow>
            0 \amp = \tan (0 + c) \implies c = 0 \amp \amp 
          </mrow>
          <mrow>
            y \amp = \tan (x) \amp \amp 
          </mrow>
        </md>
      </statement>
    </example>
  </subsection>
</section>
