<section xml:id="section-sigma-notation">
  <title>Sigma Notation</title>
  <subsection xml:id="subsection-writing-sums">
  <title>Writing Complicated Sums</title>
    <p>
      Sigma notation is a convenient way to write large and complicated
      sums. The name comes from the fact that is uses the upper case
      greek letter sigma: <m>\Sigma</m>. Sigma notation relies on an
      index and expresses the terms of the sum as expression of the
      index. In the following, <m>k</m> is the index. The term below
      the sigma tells us where the index starts and the term above the
      sigma tells us where the index ends. The term following the sigma
      is the expression of the sum: for each index from the start to the
      end (in integer steps) we evaluate the expression.
      <md>
        <mrow>
          \sum_{k=1}^5 5k \amp = 5(1) + 5(2) + 5(3) + 5(4) + 5(5) =
          5+10+15+20+25 = 75
        </mrow>
        <mrow>
          \sum_{k=1}^8 \sin \left(\frac{k\pi}{2} \right) \amp = \sin
          \left( \frac{(1)\pi}{2} \right) + \sin \left( \frac{(2)\pi}{2}
          \right) + \sin \left( \frac{(3)\pi}{2} \right) + \sin \left(
          \frac{(4)\pi}{2} \right) 
        </mrow>
        <mrow>
          \amp + \sin \left( \frac{(5)\pi}{2} \right)
          + \sin \left( \frac{(6)\pi}{2} \right) + \sin \left(
          \frac{(7)\pi}{2} \right) + \sin \left( \frac{(8)\pi}{2}
          \right)
        </mrow>
        <mrow>
          \amp = 1 + 0 + -1 + 0 + 1 + 0 + -1 + 0 = 0
        </mrow>
        <mrow>
          \sum_{k=1}^{36} k \amp = 1 + 2 + 3 + 4 + \ldots + 35 + 36 =
          666
        </mrow>
      </md>
    </p>
  </subsection>
  <subsection xml:id="subsection-manipulating-sums">
    <title>Manipulating Sums</title>
    <p>
      There are some important rules for manipulating sigma notation.
      First, sum are (unsurprisingly) linear, so we can split them up
      over addition/subtraction and pull out constants. 
    </p>
    <example>
      <statement>
        <md>
          <mrow>
            \sum_{k=1}^n 6k \amp = 6 \sum_{k=1}^n k
          </mrow>
          <mrow>
            \sum_{k=1}^n (3k^2 + 9k) \amp = 3 \sum_{k=1}^n k^2 + 9
            \sum_{k=1}^n k 
          </mrow>
        </md>
      </statement>
    </example>
    <p>
      We can combine sums if the indices match.
    </p>
    <example>
      <statement>
        <me>
          \sum_{k=1}^{15} k^2 + \sum_{k=1}^{15} 4k = \sum_{k=1}^{15}
          (k^2 + 4k)
        </me>
      </statement>
    </example>
    <p>
      If we want to combine sums when the indices don't match, we have
      to adjust the sums. There are two main methods of adjusting the
      sum. First, we can take out terms.
    </p>
    <example>
      <statement>
        <me>
          \sum_{k=1}^{15} k^2 + \sum_{k=3}^{15} 4k = 1^2 + 2^2 +
          \sum_{k=3}^{15} k^2 + \sum_{k=3}^{15} 4k = 5 + \sum_{k=3}^{15}
          (k^2 + 4k)
        </me>
      </statement>
    </example>
    <p>
      We can also shift the indices. This might seem tricky, but it's
      easy to remember if you think of balance: whatever we do to the
      index, we have to do the opposite to the expression.
    </p>
    <example>
      <statement>
        <p>
          Here we shift the index by <m>+2</m>, so the expression is
          shifted by <m>-2</m>.
          <me>
            \sum_{k=3}^{17} 4k = \sum_{k=1}^{15} 4(k+2)
          </me>
        </p>
      </statement>
    </example>
    <example>
      <statement>
        <p>
          We can use these two manipulations to combine sums if the
          indices don't initially line up.
          <me>
            \sum_{k=1}^{15} k^2 + \sum_{k=3}^{17} 4k = \sum_{k=1}^{15}
            k^2 + \sum_{k=1}^{15} 4(k+2) = \sum_{k=1}^{15} (k^2 + 4k +
            8)
          </me>
        </p>
      </statement>
    </example>
  </subsection>
  <subsection xml:id="subsection-important-sums">
    <title>Some Important Sums</title>
    <p>
      Finally, we have evaluation for some common sums. These
      expressions will be used, along with the previously stated rules,
      to calculate integrals in the next section.
      <md>
        <mrow>
          \sum_{k=1}^n 1 \amp = n
        </mrow>
        <mrow>
          \sum_{k=1}^n k \amp = \frac{n(n+1)}{2}
        </mrow>
        <mrow>
          \sum_{k=1}^n k^2 \amp = \frac{n(n+1)(2n+1)}{6}
        </mrow>
        <mrow>
          \sum_{k=1}^n k^3 \amp = \left(\frac{n(n+1)}{2} \right)^2
        </mrow>
      </md>
    </p>
    <p>
      The last sum establishes a interesting result: the sum of the
      first <m>n</m> cubes is always a square. You are welcome to check
      for yourself: the first few sums are <m>1</m>, <m>9</m>,
      <m>36</m>, <m>100</m> and <m>225</m>, all of which are square.
    </p>
  </subsection>
</section>
