<section xml:id="section-week10-activity">
  <title>Week 10 Activity</title>
  <subsection xml:id="subsection-activity-ivps">
    <title>Initial Value Problems</title>
    <activity>
      <statement>
        <p>
          Solve this initial value problem.
          <md>
            <mrow>
              \frac{dy}{dx} \amp = x^2 y^2 
              \amp \amp y(0) = 1
            </mrow>
          </md>
        </p>
      </statement>
      <solution>
        <p>
          I use the form for separable equations, with <m>f(x) =
          x^2</m> and <m>g(y) = y^2</m>.
          <me>
            \int \frac{dy}{y^2} = \int x^2 dx 
          </me>
          Then I integrate both sides, add the constant of integration
          on the right.
          <me>
            \frac{-1}{y} = \frac{x^3}{3} + c= \frac{x^3+3c}{3} 
          </me>
          Then I solve for <m>y</m>.
          <me>
            y =  \frac{-3}{x^3+3c} 
          </me>
          Now I put the initial condition values in for <m>x</m> and
          <m>y</m>, to try to solve for the constant of integration.
          <me>
            1 = \frac{-3}{x + 3c} \implies c = -1 
          </me>
          Finally, having solve for the constant of integration, I
          replace <m>c</m> with the value solved for to get the final,
          unqiue solution.
          <me>
            y = \frac{-3}{x^3 -3} = \frac{3}{3-x^3} 
          </me>
        </p>
      </solution>
    </activity>
    <activity>
      <statement>
        <p>
          Solve this initial value problem.
          <md>
            <mrow>
              \frac{dy}{dx} \amp = e^x e^{-y} 
              \amp \amp y(0) = 1 
            </mrow>
          </md>
        </p>
      </statement>
      <solution>
        <p>
          I use the form for separable equations, with <m>f(x) =
          e^x</m> and <m>g(y) = e^{-y}</m>.
          <me>
            \int e^y dy = \int e^x dx 
          </me>
          Then I integrate both sides, add the constant of integration
          on the right.
          <me>
            e^y = e^x + c 
          </me>
          Then I solve for <m>y</m>.
          <me>
            y = \ln (e^x + c) 
          </me>
          Now I put the initial condition values in for <m>x</m> and
          <m>y</m>, to try to solve for the constant of integration.
          <me>
            1 = \ln (e^0 + c) = \ln (1+c) \implies c = e-1 
          </me>
          Finally, having solve for the constant of integration, I
          replace <m>c</m> with the value solved for to get the final,
          unqiue solution.
          <me>
            y = \ln (e^x + e - 1)
          </me>
        </p>
      </solution>
    </activity>
    <activity>
      <statement>
        <p>
          Solve this initial value problem.
          <md>
            <mrow>
              \frac{dy}{dx} \amp = \frac{y}{x} 
              \amp \amp y(3) = 1
            </mrow>
          </md>
        </p>
      </statement>
      <solution>
        <p>
          I use the form for separable equations, with <m>f(x) =
          \frac{1}{x}</m> and <m>g(y) = y</m>.
          <me>
            \int \frac{1}{y} = \int \frac{1}{x} dx 
          </me>
          Then I integrate both sides, add the constant of integration
          on the right.
          <me>
            \ln |y| = \ln |x| + c 
          </me>
          Then I solve for <m>y</m>.
          <me>
            y = e^{\ln x + c} = (x)(e^c) 
          </me>
          Now I put the initial condition values in for <m>x</m> and
          <m>y</m>, to try to solve for the constant of integration.
          <me>
            1 = 3(e^c) \implies (e^c) = \frac{1}{3} \implies c = \ln
            \frac{1}{3} = -\ln 3 
          </me>
          Finally, having solve for the constant of integration, I
          replace <m>c</m> with the value solved for to get the final,
          unqiue solution.
          <me>
            y = \frac{x}{3} 
          </me>
        </p>
      </solution>
    </activity>
    <activity>
      <statement>
        <p>
          Solve this initial value problem.
          <md>
            <mrow>
              \frac{dy}{dx} \amp = \sqrt{\frac{x}{y}} 
              \amp \amp y(0) = 0 
            </mrow>
          </md>
        </p>
      </statement>
      <solution>
        <p>
          The expression in the differential equation is not defined
          for this initial value. Therefore, this IVP cannot be
          solved. I could do the separable equation, but I won't be
          able to input the initial conditions.
        </p>
      </solution>
    </activity>
    <activity>
      <statement>
        <p>
          Solve this initial value problem.
          <md>
            <mrow>
              \frac{dy}{dx} \amp = y^2 \sin x  
              \amp \amp y(\pi) = 1 
            </mrow>
          </md>
        </p>
      </statement>
      <solution>
        <p>
          I use the form for separable equations, with <m>f(x) =
          \sin x 2</m> and <m>g(y) = y^2</m>.
          <me>
            \int \frac{dy}{y^2} = \int \sin x dx 
          </me>
          Then I integrate both sides, add the constant of integration
          on the right.
          <me>
            \frac{-1}{y} = -\cos x + c 
          </me>
          Then I solve for <m>y</m>.
          <me>
            y = \frac{-1}{c - \cos x} = \frac{1}{\cos x - c} 
          </me>
          Now I put the initial condition values in for <m>x</m> and
          <m>y</m>, to try to solve for the constant of integration.
          <me>
            1 = \frac{1}{\cos \pi - c} = \frac{1}{-1 - c} \implies c= -2
          </me>
          Finally, having solve for the constant of integration, I
          replace <m>c</m> with the value solved for to get the final,
          unqiue solution.
          <me>
            y = \frac{1}{\cos x + 2}
          </me>
        </p>
      </solution>
    </activity>
    <activity>
      <statement>
        <p>
          Solve this initial value problem.
          <md>
            <mrow>
              \frac{dy}{dx} \amp = \frac{(x-1)^2}{y} 
              \amp \amp y(2) = 1 
            </mrow>
          </md>
        </p>
      </statement>
      <solution>
        <p>
          I use the form for separable equations, with <m>f(x) =
          (x-1)2</m> and <m>g(y) = \frac{1}{y}</m>.
          <me>
            \int y dy = \int (x-1)^2 dx 
          </me>
          Then I integrate both sides, add the constant of integration
          on the right.
          <me>
            \frac{y^2}{2} = \frac{(x-1)^3}{3} + c 
          </me>
          Then I solve for <m>y</m>.
          <me>
            \frac{y^2}{2} = \frac{(x-1)^3+3c}{3} \implies y =
            \sqrt{\frac{2(x-1)^3+6c}{3}} 
          </me>
          Now I put the initial condition values in for <m>x</m> and
          <m>y</m>, to try to solve for the constant of integration.
          <me>
            1 = \sqrt{\frac{2(2-1)^3+6c}{3}} \implies 1 = 2+6c \implies
            c = \frac{-1}{6}
          </me>
          Finally, having solve for the constant of integration, I
          replace <m>c</m> with the value solved for to get the final,
          unqiue solution.
          <me>
            y = \sqrt{ \frac{2(x-1)^3-1}{3}}
          </me>
        </p>
      </solution>
    </activity>
    <activity>
      <statement>
        <p>
          Solve this initial value problem.
          <md>
            <mrow>
              \frac{dy}{dx} \amp = x^3 y^4 
              \amp \amp y(1) = -3 
            </mrow>
          </md>
        </p>
      </statement>
      <solution>
        <p>
          I use the form for separable equations, with <m>f(x) =
          x^3</m> and <m>g(y) = y^4</m>.
          <me>
            \int \frac{1}{y^4} dy = \int x^3 dx 
          </me>
          Then I integrate both sides, add the constant of integration
          on the right.
          <me>
            \frac{-3}{y^3} = \frac{x^4}{4} + c = \frac{x^4 + 4c}{4}
          </me>
          Then I solve for <m>y</m>.
          <me>
            \frac{y^3}{-3} = \frac{4}{x^4 + 4x} \implies y^3 =
            \frac{-12}{x^4+4x} \implies y = \sqrt[3]{\frac{-12}{x^4 +
            4c}} 
          </me>
          Now I put the initial condition values in for <m>x</m> and
          <m>y</m>, to try to solve for the constant of integration.
          <me>
            -3 = \sqrt[3]{\frac{-12}{(1)^4+ 4c}} \implies -27 =
            \frac{-12}{1+4c} 
          </me>
          <me>
            \frac{1}{27} = \frac{1+4c}{12} \implies 1+4c =
            \frac{12}{27} \implies 4c = \frac{-15}{27} \implies c =
            \frac{-60}{27} 
          </me>
          Finally, having solve for the constant of integration, I
          replace <m>c</m> with the value solved for to get the final,
          unqiue solution.
          <me>
            y = \sqrt[3]{\frac{-12}{x^4 + \frac{-60}{27}}} =
            \sqrt[3]{\frac{324}{60 - 27x^4}} 
          </me>
        </p>
      </solution>
    </activity>
    <activity>
      <statement>
        <p>
          Solve this initial value problem.
          <md>
            <mrow>
              \frac{dy}{dx} \amp = y^2 e^x 
              \amp \amp y(\ln 3) = 2 
            </mrow>
          </md>
        </p>
      </statement>
      <solution>
        <p>
          I use the form for separable equations, with <m>f(x) =
          e^x</m> and <m>g(y) = y^2</m>.
          <me>
            \int \frac{1}{y^2} dy = \int e^x dx 
          </me>
          Then I integrate both sides, add the constant of integration
          on the right.
          <me>
            \frac{-1}{y} = e^x + c 
          </me>
          Then I solve for <m>y</m>.
          <me>
            y = \frac{-1}{e^x + c} 
          </me>
          Now I put the initial condition values in for <m>x</m> and
          <m>y</m>, to try to solve for the constant of integration.
          <me>
            2 = \frac{-1}{3+c} \implies c= \frac{-7}{2} 
          </me>
          Finally, having solve for the constant of integration, I
          replace <m>c</m> with the value solved for to get the final,
          unqiue solution.
          <me>
            y = \frac{-1}{e^x - \frac{7}{2}} = \frac{2}{7 - 2e^x} 
          </me>
        </p>
      </solution>
    </activity>
  </subsection>
  <subsection xml:id="subsection-activity-exponential-growth">
    <title>Exponential Growth</title>
    <activity>
      <statement>
        <p>
          Solve this initial value problem, where <m>p(t)</m> is
          population in terms of time. 
          <md>
            <mrow>
              \frac{dp}{dt} \amp = (0.03) p(t) 
            </mrow>
            <mrow>
              p(0) \amp = 14000
            </mrow>
          </md>
        </p>
      </statement>
      <solution>
        <p>
          I follow the process for solving separable equations, using
          <m>g(p) = p</m> and <m>f(t) = 0.03</m>. 
          <me>
            \int \frac{1}{p} dp = \int 0.03 dt 
          </me>
          I integate both sides; both a direct antiderivatives.
          <me>
            \ln |p| = 0.03t + C 
          </me>
          Then I solve for <m>p</m>. I can drop the absolute value 
          since population must be positive. 
          <me>
            p(t)  = e^{(0.03t) + C} = e^C e^{0.03t} 
          </me>
          Finally, I use the initial value p(0) = 14000.
          <me>
            p(0) = e^C e^0 = e^C = 14000
          </me>
          Here is the final solution.
          <me>
            p(t) = 14000 e^{0.03t} 
          </me>
          This is exactly what I expected: population that starts at
          14000 with a growth rate coefficient of <m>0.03</m>.
        </p>
      </solution>
    </activity>
    <activity>
      <statement>
        <p>
          Solve this initial value problem, where <m>p(t)</m> is
          population in terms of time. 
          <md>
            <mrow>
              \frac{dp}{dt} \amp = (-0.14) p(t) 
            </mrow>
            <mrow>
              p(0) \amp = 150000
            </mrow>
          </md>
        </p>
      </statement>
      <solution>
        <p>
        </p>
          I follow the process for solving separable equations, using
          <m>g(p) = p</m> and <m>f(t) = 0.03</m>. 
          <me>
            \int \frac{1}{p} dp = \int -0.14  dt 
          </me>
          I integate both sides; both a direct antiderivatives.
          <me>
            \ln |p| = (-0.14t) + C 
          </me>
          Then I solve for <m>p</m>. I can drop the absolute value 
          since population must be positive. 
          <me>
            p(t) = e^C e^{-0.14t} 
          </me>
          Finally, I use the initial value p(0) = 14000.
          <me>
            p(0) = e^C e^0 = e^C = 1500000
          </me>
          Here is the final solution.
          <me>
            p(t) = 150000 e^{-0.14t} 
          </me>
          This is exactly what I expect: population that starts at
          150000 with a growth rate coefficient of <m>-0.14</m>.
      </solution>
    </activity>
  </subsection>
  <subsection xml:id="subsection-activity-logistic-growth">
    <title>Logistic Growth</title>
    <activity>
      <statement>
        <p>
          Check that the logistic growth function given solves the
          initial value problem. <m>p(t)</m> is population in terms of
          time. (First check the initial value. Then calculate the
          right side and left side of the differential equation and
          see if you can simpify both expression into the same thing.)
          <md>
            <mrow>
              p(t) \amp = \frac{400000 e^{0.05t}}{600 + 400
              e^{0.05t}} 
            </mrow>
            <mrow>
              \frac{dp}{dt} \amp = (0.05) p(t) \left( 1 -
              \frac{p(t)}{1000} \right) 
            </mrow>
            <mrow>
              p(0) \amp = 400
            </mrow>
          </md>
        </p>
      </statement>
      <solution>
        <p>
          I have to check two things. First, I can check that the
          initial value is correct. This is simply evaluating
          <m>p(0)</m>. 
          <me>
            p(0) = \frac{400000 e^0}{600 + 400
            e^0} = \frac{400000}{600+ 400} =
            \frac{400000}{1000} = 400
          </me>
          This is the correct initial value. Now I need to
          differentiate <m>p(t)</m> using the quotient rule and check
          that it is the same as the left side of the differential
          equation. This calculation is a bit complicated with many
          pieces, but I'll simplify it step by step. 
          <md>
            <mrow>
              \frac{dp}{dt} \amp = \frac{(600 + 400e^{0.05t}) \left(
              \frac{d}{dt} 400000 e^{0.05t} \right) - 400000 e^{0.05t}
              \left( \frac{d}{dt} 600 + 400 e^{0.05t} \right)}{(600 +
              400 e^{0.05t})^2}
            </mrow>
            <mrow>
              \amp = \frac{(600 + 400e^{0.05t})((0.05)(400000)e^{0.05t} 
              - 400000 e^{0.05t}((0.05)400e^{0.05t})}{(600 + 400
              e^{0.05t})^2}
            </mrow>
            <mrow>
              \amp = \frac{(600 + 400e^{0.05t})20000 e^{0.05t} - 
              400000 e^{0.05t} 20 e^{0.05t}}{(600 + 400 e^{0.05t})^2}
            </mrow>
            <mrow>
              \amp = \frac{12000000e^{0.05t} + 8000000e^{0.1t} - 
              8000000 e^{0.1t}}{(600 + 400 e^{0.05t})^2}
            </mrow>
            <mrow>
              \amp = \frac{12000000e^{0.05t}}{(600 + 400 e^{0.05t})^2}
            </mrow>
          </md>
          After all that simplification, I have this expression. This
          is the left side of the differential equation. I want to
          compare it to the right side of the differential equation.
          I'll try to calculate that right side and see if I can
          simplify it down to the same thing. From the third to the
          fourth line below, I construct a common denominator for the
          term in brackets. 
          <md>
            <mrow>
              \amp (0.05) p(t) \left( 1 - \frac{p(t)}{1000} \right) 
            </mrow>
            <mrow>
              \amp = (0.05) \frac{400000 e^{0.05t}}{600 + 400 e^{0.05t}} 
              \left( 1 - \frac{ \frac{400000 e^{0.05t}}{600 + 400
              e^{0.05t}}}{1000} \right)
            </mrow>
            <mrow>
              \amp = \frac{20000 e^{0.05t}}{600 + 400 e^{0.05t}} 
              \left( 1 - \frac{400 e^{0.05t}}{600 + 400
              e^{0.05t}} \right)
            </mrow>
            <mrow>
              \amp = \frac{20000 e^{0.05t}}{600 + 400 e^{0.05t}} 
              \left( \frac{600 + 400 e^{0.05t} - 400
              e^{0.05t}}{600 + 400 e^{0.05t}} \right)
            </mrow>
            <mrow>
              \amp = \frac{20000 e^{0.05t}}{600 + 400 e^{0.05t}} 
              \left( \frac{600}{600 + 400 e^{0.05t}} \right)
            </mrow>
            <mrow>
              \amp = \frac{12000000 e^{0.05t}}{(600 + 400 e^{0.05t})^2} 
            </mrow>
          </md>
          This produces exactly the same expression. Both
          the left and ride sides of the equation simplify to the same
          expression. Therefore, since these simplification have made
          any actual changes to the function (just to how it is
          expressed), the right side and left side of the differential
          equation are equal, and I have confirmed that the given
          function solves the differential equation.
        </p>
      </solution>
    </activity>
    <activity>
      <statement>
        <p>
          Check that the logistic growth function given solves the
          initial value problem. <m>p(t)</m> is population in terms of
          time.
          <md>
            <mrow>
              p(t) = \frac{240000 e^{0.02t}}{-500 + 800 
              e^{0.02t}} 
            </mrow>
            <mrow>
              \frac{dp}{dt} = (0.02) p(t) \left( 1 -
              \frac{p(t)}{300} \right) 
            </mrow>
            <mrow>
              p(0) = 800
            </mrow>
          </md>
        </p>
      </statement>
      <solution>
        <p>
          I have to check two things. First, I can check that the
          initial value is correct. This is simply evaluating
          <m>p(0)</m>. 
          <me>
            p(0) = \frac{240000 e^0}{-500 + 800
            e^0} = \frac{240000}{-500+ 800} =
            \frac{240000}{300} = 800
          </me>
          This is the correct initial value. Now I need to
          differentiate <m>p(t)</m> using the quotient rule and check
          that it is the same as the left side of the differential
          equation. This calculation is a bit complicated with many
          pieces, but I'll simplify it step by step. 
          <md>
            <mrow>
              \frac{dp}{dt} \amp = \frac{(-500 + 800e^{0.02t}) \left(
              \frac{d}{dt} 240000 e^{0.02t} \right) - 240000 e^{0.02t}
              \left(\frac{d}{dt} \left( -500 + 800 e^{0.02t} \right)
              \right)}{(-500 + 800 e^{0.02t})^2}
            </mrow>
            <mrow>
              \amp = \frac{(-500 + 800e^{0.02t})(0.02)(240000)e^{0.02t} 
              - 240000 e^{0.02t}((0.02)(800)e^{0.02t})}{(-500 + 800
              e^{0.02t})^2}
            </mrow>
            <mrow>
              \amp = \frac{(-500 + 800e^{0.02t})(4800)e^{0.02t} 
              - 240000 e^{0.02t}((16)e^{0.02t})}{(-500 + 800
              e^{0.02t})^2}
            </mrow>
            <mrow>
              \amp = \frac{-6000000e^{0.02t} - 3840000e^{0.04t} 
              + 3840000 e^{0.04t}}{(-500 + 800
              e^{0.02t})^2}
            </mrow>
            <mrow>
              \amp = \frac{-6000000e^{0.02t}}{(-500 + 800
              e^{0.02t})^2}
            </mrow>
          </md>
          After all that simplification, I have this expression. This
          is the left side of the differential equation. I want to
          compare it to the right side of the differential equation.
          Let's try to calculate that right side and see if I can
          simplify it down to the same thing. From the third to the
          fourth line below, I construct a common denominator for the
          term in brackets.
          <md>
            <mrow>
              \amp (0.02) p(t) \left( 1 - \frac{p(t)}{300} \right) 
            </mrow>
            <mrow>
              \amp = (0.02) \frac{240000 e^{0.02t}}{-500 + 800 e^{0.02t}} 
              \left( 1 - \frac{ \frac{240000 e^{0.02t}}{-500 + 800
              e^{0.02t}}}{300} \right)
            </mrow>
            <mrow>
              \amp = \frac{12000 e^{0.02t}}{-500 + 800 e^{0.02t}} 
              \left( 1 - \frac{800 e^{0.02t}}{-500 + 800 e^{0.02t}}
              \right)
            </mrow>
            <mrow>
              \amp = \frac{12000 e^{0.02t}}{-500 + 800 e^{0.02t}} 
              \left( \frac{-500 + 800e^{0.02t} - 800 e^{0.02t}}{-500 +
              800 e^{0.02t}} \right)
            </mrow>
            <mrow>
              \amp = \frac{12000 e^{0.02t}}{-500 + 800 e^{0.02t}} 
              \left( \frac{-500}{-500 + 800 e^{0.02t}} \right)
            </mrow>
            <mrow>
              \amp = \frac{-6000000 e^{0.02t}}{(-500 + 800
              e^{0.02t})^2} 
            </mrow>
          </md>
          This produces exactly the same expression. Both
          the left and ride sides of the equation simplify to the same
          expression. Therefore, since these simplification have made
          any actual changes to the function (just to how it is
          expressed), the right side and left side of the differential
          equation are equal, and I have confirmed that the given
          function solves the differential equation.
        </p>
      </solution>
    </activity>
  </subsection>
  <subsection xml:id="subsection-week10-concepts">
    <title>Conceptual Review Questions</title>
    <p>
      <ul>
        <li>
          How are exponential growth and logistic growth encoded in
          differential equations?
        </li>
        <li>
          What does it mean to solve a differential equation?
        </li>
        <li>
          What is an initial condition and why do I need them to
          solve differential conditions?
        </li>
      </ul>
    </p>
  </subsection>
</section>
