<section xml:id="des">
  <title>Solving Differential Equations</title>
  <subsection xml:id="direct-integration">
    <title>Solving By Direct Integration</title>
    <p>
      Early in the course,
      we talked about differential equations in order to understand derivatives as rates of changes.
      We looked at autonomous differential equations,
      particularly for populations models,
      and we used the qualitative technique of phase-line analysis to understand them.
    </p>
    <p>
      Now that we can calculate derivatives and integrals in some detail,
      we can return to differential equations.
      With these techniques,
      we'll actually try to solve the DEs, instead of using a qualitative approach.
      In the easiest case,
      the right side of a DE only involves the independant variable.
      <me>
        \frac{df}{dx} = g(x)
      </me>
    </p>
    <p>
      Since only the independant variable <m>x</m> appears on the right side,
      we can simply integrate both sides in <m>x</m>.
      <me>
        \int \frac{df}{dx} dx = \int g(x) dx
      </me>
    </p>
    <p>
      On the left,
      the integral of the derivative is the original funciton <m>f</m>.
      <me>
        f(x) = \int g(x) dx
      </me>
    </p>
  </subsection>
  <subsection xml:id="ivps">
    <title>Initial Value Problems</title>
    <p>
      When we integrate to solve a DE, we will get a constant of integration.
      In order to determine that constant,
      we are often given an initial condition, such as <m>f(0) = 0</m>.
      Differential equations problems with initial conditions are often called
      <em>initial value problems</em> (IVPs).
    </p>
    <example>
      <statement>
        <md>
          <mrow>\frac{df}{dx} \amp  = x^3   f(0) = 7</mrow>
          <mrow>\int \frac{df}{dx} \amp  = \int x^3 dx</mrow>
          <mrow>f \amp  = \frac{x^4}{4} + c</mrow>
          <mrow>7 \amp  = \frac{0^4}{4} + c \implies c = 7</mrow>
          <mrow>f(x) \amp  = \frac{x^4}{4} + 7</mrow>
        </md>
      </statement>
    </example>
    <example>
      <statement>
        <md>
          <mrow>\frac{df}{dx} \amp  = 6 \sin 3t   f \left( \frac{\pi}{6}
          \right) = 6</mrow>
          <mrow>f(x) \amp  = \int 6 \sin 3t dt = -2\cos 3x + c</mrow>
          <mrow>6 \amp  = -2\cos \frac{\pi}{2} + c = 0 + c \implies c=6</mrow>
          <mrow>f(x) \amp  = -2 \cos 3x + 6</mrow>
        </md>
      </statement>
    </example>
    <example>
      <statement>
        <md>
          <mrow>\frac{df}{dx} \amp  = \frac{1}{x^2+1}   f(1) = \pi</mrow>
          <mrow>f \amp  = \int \frac{1}{x^2+1} dx = \arctan x + c</mrow>
          <mrow>\pi \amp  = \arctan(1) + c = \frac{\pi}{4} + c \implies c =
          \frac{3\pi}{4}</mrow>
          <mrow>f(x) \amp  = \arctan x + \frac{3\pi}{4}</mrow>
        </md>
      </statement>
    </example>
  </subsection>
  <subsection xml:id="seperable">
    <title>Seperable Differential Equations</title>
    <p>
      Solving DEs is a very difficult task is general;
      the previous examples were all artificially simple.
      For this course,
      we're going to restrict to a specific type of DE called a seperable equation.
      Let <m>f(x)</m> and <m>g(y)</m> be continuous functions in <m>x</m> and <m>y</m>,
      respectively.
      Seperable differential equations are DEs where the dependent and independent variable can be seperated.
      <me>
        \frac{dy}{dx} = f(x) g(y)
      </me>
    </p>
    <p>
      In particular,
      this includes the autonomous equations we previously studied;
      if we set <m>f=1</m> then we get an autonomous equation.
    </p>
    <p>
      To solve these equations,
      take <m>g(y)</m> to the left side of the equation and then integrate in <m>x</m>.
      <md>
        <mrow>\frac{1}{g(y)} \frac{dy}{dx} \amp  = f(x)</mrow>
        <mrow>\int \frac{1}{g(y)} \frac{dy}{dx} dx \amp  = f(x) dx</mrow>
      </md>
    </p>
    <p>
      With a substitution,
      we can change the left side of the integral into an integral in <m>y</m>.
      <me>
        \int \frac{1}{g(y)} dy = \int f(x) dx
      </me>
    </p>
    <p>
      To remember this set up,
      often we abuse Leibniz notation and pretend that
      <m>\frac{dy}{dx}</m> is a fraction of infinitesimals.
      If we do this,
      all we need to do is isolate <m>g(y)</m> with <m>y</m> on the left and <m>f(x)</m> with <m>dx</m> on the right,
      then integrate.
      <md>
        <mrow>\frac{dy}{dx} \amp  = f(x) g(y)</mrow>
        <mrow>\frac{1}{g(y)} dy \amp  = f(x) dx</mrow>
        <mrow>\int \frac{1}{g(y)} dy \amp  = \int f(x) dx</mrow>
      </md>
    </p>
    <p>
      Finally, after the integration is complete,
      we try to solve for <m>y</m> as a function of <m>x</m>.
      If we can, that function is the solution.
      Often we can't, and we leave the result as an implicit expression in <m>x</m> and <m>y</m>.
    </p>
    <example>
      <statement>
        <md>
          <mrow>\frac{dy}{dx} \amp  = \frac{\sin x}{y}</mrow>
          <mrow>y dy \amp  = \sin x dx</mrow>
          <mrow>\frac{y^2}{2} \amp  = - \cos x + c</mrow>
          <mrow>y \amp  = \pm \sqrt{c - 2\cos x}</mrow>
          <mrow>\text{ Initial condition: }  y(0) \amp  = 1</mrow>
          <mrow>1 \amp  = \sqrt{c - 2 \cos (0)} = \sqrt{c-2}</mrow>
          <mrow>1 \amp  = c-2</mrow>
          <mrow>c \amp  = 3</mrow>
          <mrow>y \amp  = \sqrt{3 - 2 \cos x}</mrow>
        </md>
      </statement>
    </example>
    <example>
      <statement>
        <md>
          <mrow>\frac{dy}{dx} \amp  = \frac{-x}{y}</mrow>
          <mrow>\int y dy \amp  = - \int x dx</mrow>
          <mrow>\frac{y^2}{2} \amp  = \frac{-x^2}{2} + c</mrow>
          <mrow>y^2 + x^2 \amp  = c</mrow>
          <mrow>\text{ Initial condition: }  y(4) \amp  = 3</mrow>
          <mrow>4^2 + 3^2 \amp  = c</mrow>
          <mrow>c \amp  = 25</mrow>
          <mrow>y^2 + x^2 \amp  = 25</mrow>
        </md>
        <p>
          There is no way to solve for <m>y</m> as a function of <m>x</m>,
          so we leave this as an implicit expression in both variables.
        </p>
      </statement>
    </example>
    <example>
      <statement>
        <md>
          <mrow>\frac{dy}{dx} \amp  = y^2 - 4</mrow>
          <mrow>\int \frac{1}{y^2-4} dy \amp  = \int 1 dx</mrow>
          <mrow>\frac{-1}{2} \arctanh \left( \frac{y}{2} \right) \amp  = x + c</mrow>
          <mrow>\arctanh \left( \frac{y}{2} \right) \amp  = -2x + c</mrow>
          <mrow>\frac{y}{2} \amp  = \tanh (-2x + c)</mrow>
          <mrow>y \amp  = 2 \tanh (-2x + c)</mrow>
          <mrow>\text{ Initial condition: }  y(0) \amp  = 0</mrow>
          <mrow>0 \amp  = 2 \tanh (0 + c)</mrow>
          <mrow>c \amp  = 0</mrow>
          <mrow>y \amp  = 2 \tanh (-2x)</mrow>
        </md>
      </statement>
    </example>
  </subsection>
</section>